lean/Eternity2/Puzzle.lean
@@ -1,5 +1,4 @@
 import Eternity2.Puzzle.Board
-import Eternity2.Puzzle.ColorCardConstraints
 import Eternity2.Puzzle.EdgeConstraints
 import Eternity2.Puzzle.GenBoard
 import Eternity2.Puzzle.SolvePuzzle
